FormaleSystemeInLean/LectureAndExercise/lecture4.lean
@@ -1,0 +1,64 @@
+import FormaleSystemeInLean.LectureAndExercise.lecture1
+
+structure NFA (Q : Type u) (Sigma : Type v) [Fintype Q] [Fintype Sigma] where
+  δ: Q -> Sigma → List Q
+  Q0 : List Q
+  F : List Q
+
+variable {Q : Type u} {Sigma : Type v} [Fintype Q] [Fintype Sigma] [Fintype (Option Q)]
+
+def NFA.δ_word (nfa : NFA Q Sigma) (R : List Q) : (Word Sigma) → List Q
+  | .nil => R
+  | .cons a v => nfa.δ_word (R.flatMap (nfa.δ · a)) v
+
+inductive NFA.Run (nfa : NFA Q Sigma) : Q -> Q -> Word Sigma -> Type _
+| self (q : Q) : nfa.Run q q []
+| step {q1 q2 qf : Q} {a : Sigma} {v : Word Sigma} (r : nfa.Run q2 qf v) (q2_mem : q2 ∈ nfa.δ q1 a) : nfa.Run q1 qf (a :: v)
+
+def NFA.Run.from_start {nfa : NFA Q Sigma} (_ : nfa.Run q0 q w) : Prop := q0 ∈ nfa.Q0
+def NFA.Run.accepts {nfa : NFA Q Sigma} (_ : nfa.Run q qf w) : Prop := qf ∈ nfa.F
+
+def NFA.Language (nfa : NFA Q Sigma) : Language Sigma :=
+  fun w => ∃ (q0 qf : Q) (r : nfa.Run q0 qf w), r.from_start ∧ r.accepts
+
+-- soll in
+theorem run_imp_mem_δ (nfa : NFA Q Sigma) (q1 qn : Q) (R : List Q) (w : Word Sigma) : nfa.Run q1 qn w → q1 ∈ R → qn ∈ nfa.δ_word R w := by
+  intro r q1_mem
+  -- induktion über den lauf
+  induction w generalizing q1 R with
+  | nil =>
+    unfold NFA.δ_word
+    have eq : q1 = qn := by
+      cases r; rfl
+    subst eq
+    exact q1_mem
+  | cons a v ih =>
+    cases r with
+    | @step run mem q_a q_b q_c x y =>
+      have no_idea : qn ∈ nfa.δ_word (nfa.δ q1 a) v := by
+        apply ih _ (nfa.δ q1 a) x y
+      simp only [NFA.δ_word]
+      have idk : q1 ∈ R → nfa.δ q1 a ⊆ nfa.δ_word R [a] := by
+        intro q_mem q' q1_mem_δ
+        unfold NFA.δ_word
+
+        sorry
+      sorry
+
+theorem acc_run_iff_δ_word_contains_final (nfa : NFA Q Sigma) (w : Word Sigma) : w ∈ nfa.Language ↔ ∃ q ∈ nfa.δ_word nfa.Q0 w, q ∈ nfa.F := by
+  constructor
+  . intro w_mem
+    rcases w_mem with ⟨q0, qf, r, r_s, r_acc⟩
+    unfold NFA.Run.accepts at r_acc
+    unfold NFA.Run.from_start at r_s
+    exists qf
+
+    constructor
+    . sorry
+
+    . sorry
+  . intro h
+    unfold NFA.Language
+    simp only [Membership.mem]
+
+    sorry
